theories/L/Complexity/Problems/kSAT.v
@@ -6,36 +6,36 @@ From Undecidability.L.Datatypes Require Import LProd LTerm LLNat LLists LOptions
 
 Inductive kCNF (k : nat) : cnf -> Prop :=
 | kCNFB : kCNF k []
-| kCNFS (c : cnf) (cl : clause) : (|cl|) = k -> kCNF k c -> kCNF k (cl :: c).               
+| kCNFS (N : cnf) (C : clause) : (|C|) = k -> kCNF k N -> kCNF k (C ::  N).               
 
 Hint Constructors kCNF.
 
-Lemma kCNF_clause_length (k : nat) (c : cnf) : kCNF k c <-> forall cl, cl el c -> |cl| =k.
+Lemma kCNF_clause_length (k : nat) (N : cnf) : kCNF k N <-> forall C, C el N -> |C| =k.
 Proof.
   split. 
   - induction 1. 
-    + intros cl [].
-    + intros cl' [-> | Hel]; [assumption | now apply IHkCNF]. 
-  - intros H. induction c; [eauto | ].
-    constructor; [now apply H | apply IHc; eauto].
+    + intros C [].
+    + intros C' [-> | Hel]; [assumption | now apply IHkCNF]. 
+  - intros H. induction N; [eauto | ].
+    constructor; [now apply H | apply IHN; eauto].
 Qed. 
 
-Lemma kCNF_app (k : nat) (c1 c2 : cnf) : kCNF k (c1 ++ c2) <-> kCNF k c1 /\ kCNF k c2. 
+Lemma kCNF_app (k : nat) (N1 N2 : cnf) : kCNF k (N1 ++ N2) <-> kCNF k N1 /\ kCNF k N2. 
 Proof. 
-  induction c1; cbn; split. 
+  induction N1; cbn; split. 
   - eauto.
   - tauto.
-  - intros H. inv H. apply IHc1 in H3 as (H3 & H4). split; eauto.
-  - intros [H1 H2]. inv H1. constructor; [easy | ]. now apply IHc1. 
+  - intros H. inv H. apply IHN1 in H3 as (H3 & H4). split; eauto.
+  - intros [H1 H2]. inv H1. constructor; [easy | ]. now apply IHN1. 
 Qed. 
 
-Definition kSAT (k : nat) (c : cnf) : Prop := k > 0 /\ kCNF k c /\ SAT c. 
+Definition kSAT (k : nat) (N : cnf) : Prop := k > 0 /\ kCNF k N /\ SAT N. 
 
 (** boolean decider for kCNF *)
-Definition clause_length_decb (k : nat) := (fun (cl : clause) => Nat.eqb k (|cl|)).
-Definition kCNF_decb (k : nat) (c : cnf) := forallb (clause_length_decb k) c. 
+Definition clause_length_decb (k : nat) := (fun (C : clause) => Nat.eqb k (|C|)).
+Definition kCNF_decb (k : nat) (N : cnf) := forallb (clause_length_decb k) N. 
 
-Lemma kCNF_decb_iff (k : nat) (c : cnf) : kCNF_decb k c = true <-> kCNF k c. 
+Lemma kCNF_decb_iff (k : nat) (N : cnf) : kCNF_decb k N = true <-> kCNF k N. 
 Proof.
   rewrite kCNF_clause_length. unfold kCNF_decb, clause_length_decb. 
   rewrite forallb_forall. setoid_rewrite Nat.eqb_eq. firstorder.
@@ -46,16 +46,15 @@ From Undecidability.L.Tactics Require Import LTactics GenEncode.
 From Undecidability.L.Complexity Require Import PolyBounds. 
 
 Definition c__clauseLengthDecb :=  c__length + c__nat_eqb2 + 1.
-Definition clause_length_decb_time (k : nat) (cl : clause) := c__length * (|cl|) + nat_eqb_time k (|cl|) + c__clauseLengthDecb.
-Instance term_clause_length_decb : computableTime' clause_length_decb (fun k _ => (1, fun cl _ => (clause_length_decb_time k cl, tt))). 
+Definition clause_length_decb_time (k : nat) (C : clause) := c__length * (|C|) + nat_eqb_time k (|C|) + c__clauseLengthDecb.
+Instance term_clause_length_decb : computableTime' clause_length_decb (fun k _ => (1, fun C _ => (clause_length_decb_time k C, tt))). 
 Proof. 
   extract. solverec. unfold clause_length_decb_time, c__clauseLengthDecb. solverec. 
 Defined. 
 
-
 Definition c__kCNFDecb := 3. 
-Definition kCNF_decb_time (k : nat) (c : cnf) := forallb_time (fun cl => clause_length_decb_time k cl) c + c__kCNFDecb.
-Instance term_kCNF_decb : computableTime' kCNF_decb (fun k _ => (1, fun c _ => (kCNF_decb_time k c, tt))). 
+Definition kCNF_decb_time (k : nat) (N : cnf) := forallb_time (fun C => clause_length_decb_time k C) N + c__kCNFDecb.
+Instance term_kCNF_decb : computableTime' kCNF_decb (fun k _ => (1, fun N _ => (kCNF_decb_time k N, tt))). 
 Proof. 
   extract. solverec. unfold kCNF_decb_time, c__kCNFDecb. solverec. 
 Defined. 
@@ -63,12 +62,12 @@ Defined.
 Definition c__kCNFDecbBound1 := c__length + c__nat_eqb.
 Definition c__kCNFDecbBound2 := c__clauseLengthDecb + c__forallb + c__kCNFDecb.
 Definition poly__kCNFDecb n := (n + 1) * (c__kCNFDecbBound1 * (n + 1)  + c__kCNFDecbBound2). 
-Lemma kCNF_decb_time_bound k c : kCNF_decb_time k c <= poly__kCNFDecb (size (enc c) + size (enc k)). 
+Lemma kCNF_decb_time_bound k N : kCNF_decb_time k N <= poly__kCNFDecb (size (enc N) + size (enc k)). 
 Proof. 
   unfold kCNF_decb_time. rewrite forallb_time_bound_env.
   2: { 
     split. 
-    - intros cl n. unfold clause_length_decb_time. 
+    - intros C n. unfold clause_length_decb_time. 
       rewrite nat_eqb_time_bound_r. rewrite list_size_length at 1. rewrite list_size_enc_length. 
       instantiate (1 := registered_nat_enc).
       instantiate (1 := fun n => (c__length + c__nat_eqb) * (n + 1) + c__clauseLengthDecb). 
