theories/L/Complexity/Reductions/kSAT_to_SAT.v
@@ -1,54 +1,51 @@
 From Undecidability.L.Complexity Require Import NP Synthetic Problems.SAT Problems.Clique. 
 From Undecidability.L Require Import Tactics.LTactics.
-From Undecidability.L.Complexity Require Import Problems.kSAT PolyBounds Tactics NP. 
-From Undecidability.L.Datatypes Require Import LBool LNat Lists LProd. 
+From Undecidability.L.Complexity Require Import Problems.kSAT PolyBounds NP Synthetic. 
+From Undecidability.L.Datatypes Require Import LBool LLNat LLists LProd. 
 
-Lemma evalCnf_inv_true (c : cnf) (cl :clause) (a : assgn) : (evalCnf a (cl::c) = Some true) -> (evalCnf a c = Some true). 
-  intros (b1 & b2 & H1 & H2 & H3)%evalCnf_step_inv. 
-  simp_bool. 
-Qed. 
-
-Lemma ksat_to_sat (k : nat): reducesPolyMO (kSAT k) SAT. 
+Lemma kSAT_to_SAT (k : nat): reducesPolyMO (unrestrictedP (kSAT k)) (unrestrictedP SAT). 
 Proof. 
+  destruct k. 
+  { (* always return a trivial no-instance if k = 0 *)
+    apply reducesPolyMO_intro with (f := fun N => [[(true, 0)]; [(false, 0)]]).  
+    - exists (fun n => 13).
+      + extract. solverec. 
+      + smpl_inO. 
+      + smpl_inO. 
+      + exists (fun n => size (enc [[(true, 0)]; [(false, 0)]])); [solverec | smpl_inO | smpl_inO].
+    - intros N ?. cbn. exists Logic.I. unfold kSAT. 
+      split; [lia | ]. intros [a H]. 
+      unfold satisfies, evalCnf, evalCnf_step in H; cbn in H. 
+      destruct evalVar; cbn in H; congruence. 
+  } 
+
   (*check if it is a kCNF. if so, the reduction the SAT instance is the identity. otherwise, return a negative SAT instance*)
-  exists (fun x => if kCNF_decb k x then x else [[(true, 0)]; [(false, 0)]] ). 
-  split.
-  - specialize (kCNF_decb_time_bound) as (f' & H1 & H2 & H3). 
-    evar (f : nat -> nat). exists f.
-    + constructor. extract. solverec; rewrite H1. 
-      instantiate (f:= fun n => f' n + 17). all: subst f; solverec. 
-    + subst f; smpl_inO. 
-    + subst f; smpl_inO. 
-    + (* now we need to prove that the output of the reduction is polynomial *)
-        evar (tf : nat -> nat). exists tf. split. 
-        1 : {
-          intros x. destruct (kCNF_decb k x).
-          Compute (size(enc [[(true, 0)]; [(false, 0)]])).
-          instantiate (tf := fun n => n + 55).
-          all: subst tf. 2 : replace (size(enc [[(true, 0)]; [(false, 0)]])) with 55. 1-2: lia.
-          now cbv.
-        }
-        split; subst tf; smpl_inO. 
-  - intros x. split.
-    + intros ( H1 & a & H2). destruct (kCNF_decb k x) eqn:H3. now exists a. clear H2. 
-      induction H1. 
-      * unfold kCNF_decb in H3; simp_bool. rewrite Nat.leb_nle in H3. lia. cbn in H3; congruence.
-      * specialize (kCNF_decb_correct k c) as H4.
-        cbn in H3. simp_bool.
-        -- unfold kCNF_decb_pred in H3. unfold kCNF_decb in H3. simp_bool. rewrite Nat.leb_nle in H3.
-           apply kCNF_kge in H1; lia. cbn in H3; simp_bool. unfold kCNF_decb_pred in H3. 
-           now apply beq_nat_false in H3. apply IHkCNF. unfold kCNF_decb. simp_bool; right; apply H3. 
-    + intros (a & H). destruct (kCNF_decb k x) eqn:H1. split. rewrite kCNF_decb_correct in H1. 
-      induction x; constructor.
-      * tauto. 
-      * symmetry. apply H1. now left. 
-      * apply IHx. split; try tauto. intros cl H2. apply H1. now right. now apply evalCnf_inv_true with (cl:= a0). 
-      * now exists a. 
-      * destruct a. now cbn in H. destruct b; cbn in H; congruence.
+  apply reducesPolyMO_intro with (f := fun N => if kCNF_decb (S k) N then N else [[(true, 0)]; [(false, 0)]]) . 
+  - evar (f : nat -> nat). exists f. 
+    + extract. solverec.
+      all: rewrite kCNF_decb_time_bound. 
+      instantiate (f := fun n => poly__kCNFDecb (n + size (enc (S k))) + 18). 
+      all: subst f; solverec. 
+    + subst f; smpl_inO. apply inOPoly_comp; smpl_inO; apply kCNF_decb_poly. 
+    + subst f; smpl_inO. apply kCNF_decb_poly. 
+    + evar (g : nat -> nat). exists g. 
+      * intros N. destruct kCNF_decb. 
+        instantiate (g := fun n => n + size (enc [[(true, 0)]; [(false, 0)]])). 
+        all: subst g; solverec. 
+      * subst g; smpl_inO. 
+      * subst g; smpl_inO. 
+  - intros N ?. cbn. exists Logic.I. split.
+    + intros [H1 [H2 H3]].
+      apply kCNF_decb_iff in H2. rewrite H2. apply H3.  
+    + destruct kCNF_decb eqn:H1. 
+      * apply kCNF_decb_iff in H1. intros H2. split; [lia | split; easy]. 
+      * intros [a H]. unfold satisfies, evalCnf, evalCnf_step in H; cbn in H. 
+      destruct evalVar; cbn in H; congruence. 
 Qed. 
 
-Lemma inNP_kSAT (k : nat) : inNP (kSAT k). 
+Lemma inNP_kSAT (k : nat) : inNP (unrestrictedP (kSAT k)). 
 Proof.
-  apply red_inNP with (regY := @registered_list_enc (list (bool * nat)) (@registered_list_enc (bool * nat)(@registered_prod_enc bool nat  registered_bool_enc registered_nat_enc) ))(Q := SAT). 
-  apply ksat_to_sat. apply sat_NP. 
+  eapply red_inNP with (Q := unrestrictedP SAT). 
+  - apply kSAT_to_SAT. 
+  - apply sat_NP. 
 Qed. 
